%27 de marzo
We continue with the ART method. 
\subsection{Row action Form}
$k$-th iteration. Sweeps through the rows of $A$ which update $x^{(k-1)} \to x^{(n)}$. i.e. for $j=1,2,\ldots$
$$x^{(k)} = x^{(k-1)} + \frac{b_j - a^T_j x^{(k-1)}}{a^T_j a_j} a_j$$
\underline{Algorithm} (geometric Interpretation)
\begin{enumerate}[1)]
\item Take the $j$th row of A.
\item Turn it into a vector in $\RRR^n$. Note; can compute $|a_j|$ ahead of time.
\item Project orthogonally previous solution onto hyperplane $\{z: \  a^T_j z = b_j\}$
\end{enumerate}

\begin{teorema}
If $A$ is a square and non-singular matrix, then:
$$\left| A^{-1}b - x^{(k)_i} \right|_2^2 = \left| A^{-1}b - x^{(k)_{i-1}} \right|_2 - (b_i - a^T_i x^{(k)_{i-1}})^2$$
$\implies$ resigual norm is non-increasing.
\end{teorema}

\begin{teorema}
$a_i$ is rich in some components related to left singular vectors. \\
$\theta_{ij}=$ angle between $a_i$ and $v_j$ from:
$$\cos \theta_{ij} = \frac{a_i^T v_j}{|a_i|} = \frac{a^T_i}{|a_i|} v_j$$
then substituting $a_i^T v_j = e^T_i A v_j$  one gets:
$$\frac{e^T_i A v_j}{|a_i|} = \frac{\sigma_j e^T_i u_j}{|a_i|} = \frac{\sigma_j u_{ij}}{|a_i|}$$
\end{teorema}

\begin{ddef}
The Krylow Subspace is defined as:
$$\K_k(A^TA,Ab) = \spann\{A^Tb  , (A^TA)A^Tb, \ldots, (A^TA)^{k-1} A^Tb\}$$
$\dim \K_k \leq k$
\end{ddef}
method is fundamentally going to:
\begin{gather*}
A^Tb = \omega_j \quad \omega_i \frac{\omega_i}{|\omega_i|} \quad \K_1\\
\text{the second subspace}\\
(A^TA)\omega_1 = \hat \omega_2, \quad \tilde \omega_2 = \hat \omega_2 - (\omega_1^T\hat \omega_2) \omega_1, \quad \omega_2  =\frac{\omega_2}{|\omega_2|} \\
\text{ the third subspace}
(A^TA)\omega_2 = \hat \omega_3, \quad \tilde \omega_3 = \hat \omega_3 - (\omega_2^T\hat \omega_3) \omega_2, \quad \omega_3  =\frac{\omega_3}{|\omega_3|} \\
\omega_k = [\omega_1,\ldots, \omega_k ] _{n\times k}
\end{gather*}

$x^{(k)} \in \K_k \iff x^{(k) } $ linear combination of $\omega_1, \omega_2 , \ldots, \omega_k$.\\
Then we can write $x^{(k)} = \omega_k \xi _k$ and:
\begin{gather*}
A^TAx= A^Tb\\
((A^TA)w_k)\xi_k = A^Tb
\end{gather*}
